Progress

compiler/backend/proofs/source_evalProofScript.sml
@@ -45,11 +45,9 @@ Definition do_eval_record_def:
     | _ => NONE
 End
 
-
-
-(* non-Eval case. it's almost straightforward except Envs might be
-   represented differently, which means we need a v_rel, and to assume
-   no Rtype_error, etc, which is sad *)
+(* the non-Eval case. we need to prove that if there are (syntactically)
+   no Eval ops, this will always be the case, and so we can replace an
+   activated EvalDecs eval state with NONE *)
 
 Definition env_rel_def:
   env_rel v_rel (env : v sem_env) env' <=>
@@ -101,87 +99,14 @@ Proof
   \\ fs []
   \\ res_tac
 QED
+
+Theorem env_rel_nsEmpty = LIST_CONJ
+  [Q.SPECL [`R`, `x with <| v := nsEmpty |>`] env_rel_def,
+    Q.SPECL [`R`, `x`, `y with <| v := nsEmpty |>`] env_rel_def]
+  |> SIMP_RULE (std_ss ++ simpLib.type_ssfrag ``: 'a sem_env``)
+        [nsLookup_nsEmpty]
+
 val _ = IndDefLib.add_mono_thm env_rel_mono_rel;
-
-Inductive no_Eval_v_rel:
-  (no_Eval_v_rel (Env env) v) /\
-  (LIST_REL no_Eval_v_rel xs ys ==>
-    no_Eval_v_rel (Vectorv xs) (Vectorv ys)) /\
-  (LIST_REL no_Eval_v_rel xs ys ==>
-    no_Eval_v_rel (Conv stmp xs) (Conv stmp ys)) /\
-  (env_rel no_Eval_v_rel env env' ==>
-    no_Eval_v_rel (Closure env nm x) (Closure env' nm x)) /\
-  (env_rel no_Eval_v_rel env env' ==>
-    no_Eval_v_rel (Recclosure env funs nm) (Recclosure env' funs nm)) /\
-  (no_Eval_v_rel (Litv l) (Litv l)) /\
-  (no_Eval_v_rel (Loc n) (Loc n))
-End
-
-Theorem no_Eval_v_rel_l_cases =
-  [``no_Eval_v_rel (Litv l) v``, ``no_Eval_v_rel (Conv cn vs) v``,
-    ``no_Eval_v_rel (Loc l) v``, ``no_Eval_v_rel (Vectorv vs) v``,
-    ``no_Eval_v_rel (Env e) v``,
-    ``no_Eval_v_rel (Recclosure env funs nm) v``,
-    ``no_Eval_v_rel (Closure env nm x) v``]
-  |> map (SIMP_CONV (srw_ss ()) [Once no_Eval_v_rel_cases])
-  |> map GEN_ALL
-  |> LIST_CONJ
-
-Theorem no_Eval_v_rel_Boolv:
-  (no_Eval_v_rel (Boolv b) v) = (v = Boolv b)
-Proof
-  rw [Boolv_def, no_Eval_v_rel_l_cases]
-QED
-
-Definition no_Eval_s_rel_def:
-  no_Eval_s_rel s s' <=>
-  ?es refs. s' = s with <| refs := refs;
-    eval_state := SOME (EvalOracle es) |> /\
-  LIST_REL (sv_rel no_Eval_v_rel) s.refs refs /\
-  s.eval_state = SOME EvalDecs
-End
-
-val s = mk_var ("s", ``: 'ffi semanticPrimitives$state``);
-
-fun do_match_inst const data thm = let
-    val (vs, t1) = strip_forall (concl thm)
-    val (lhs, _) = dest_imp t1
-    val vset = HOLset.addList (empty_tmset, vs)
-    val mem_vset = curry HOLset.member vset
-    fun match_vars_free ("m", t) = all (not o mem_vset) (free_vars t)
-      | match_vars_free _ = true
-    fun inst_var ("i", t) = exists mem_vset (free_vars t)
-      | inst_var _ = false
-    val prems = strip_conj lhs
-      |> filter (same_const const o fst o strip_comb)
-      |> filter (all match_vars_free o zip data o snd o strip_comb)
-      |> filter (exists inst_var o zip data o snd o strip_comb)
-  in MAP_FIRST (fn prem => let
-    val const = strip_comb prem |> fst
-    val prem_els = strip_comb prem |> snd |> zip data
-    fun matches (("m", t), t') = term_eq t t'
-      | matches _ = true
-    fun assum_match a = case strip_comb a of (c, xs) =>
-      term_eq c const andalso all matches (zip prem_els xs)
-  in FIRST_ASSUM (fn a => if assum_match (concl a)
-  then let
-    val fvs = FVL [concl thm, concl a] empty_tmset
-    val (vs2, sub) = quantHeuristicsTools.list_variant (HOLset.listItems fvs) vs
-    val thm2 = SPECL vs2 thm
-    val prem2 = subst sub prem
-    val els2 = strip_comb prem2 |> snd |> zip data
-    fun get_subst (("i", t), t') = fst (match_term t t')
-      | get_subst _ = []
-    val sub2 = strip_comb (concl a) |> snd |> zip els2
-      |> map get_subst |> List.concat
-    val thm3 = INST sub2 thm2
-    val fvs2 = FVL [concl thm3] empty_tmset
-    val vs3 = filter (curry HOLset.member fvs2) vs2
-    val thm4 = GENL vs3 thm3
-  in assume_tac thm4 end
-  else NO_TAC)
-  end) prems
-  end
 
 Inductive no_Eval_v:
   (no_Eval_v (Env env)) /\
@@ -199,7 +124,7 @@ Definition no_Eval_env_def:
   no_Eval_env env = env_rel (\x y. no_Eval_v x) env env
 End
 
-Theorem no_Eval_v_cases =
+Theorem no_Eval_v_simps =
   [``no_Eval_v (Litv l)``, ``no_Eval_v (Conv cn vs)``,
     ``no_Eval_v (Loc l)``, ``no_Eval_v (Vectorv vs)``,
     ``no_Eval_v (Env e)``,
@@ -209,13 +134,16 @@ Theorem no_Eval_v_cases =
   |> map GEN_ALL
   |> LIST_CONJ
 
+(* is there a [simp local] type way to do this? *)
+val _ = bossLib.augment_srw_ss [rewrites [no_Eval_v_simps]];
+
 Theorem do_opapp_no_Eval:
   do_opapp vs = SOME (env, v) /\
   EVERY no_Eval_v vs ==>
   no_Eval_env env /\ ~ has_Eval v
 Proof
   rw [do_opapp_cases]
-  \\ fs [no_Eval_v_cases, no_Eval_env_def]
+  \\ fs [no_Eval_env_def]
   >- (
     irule env_rel_add_nsBind
     \\ simp []
@@ -227,7 +155,7 @@ Proof
     \\ simp []
     \\ irule EVERY2_refl
     \\ fs [MEM_MAP, FORALL_PROD, EXISTS_PROD, PULL_EXISTS]
-    \\ simp [quotient_pairTheory.PAIR_REL_THM, no_Eval_v_cases, no_Eval_env_def]
+    \\ simp [quotient_pairTheory.PAIR_REL_THM, no_Eval_env_def]
   )
   >- (
     fs [find_recfun_ALOOKUP, EVERY_MEM, MEM_MAP, EXISTS_PROD, PULL_EXISTS]
@@ -240,15 +168,15 @@ Theorem no_Eval_v_list_to_v:
   !xs. no_Eval_v (list_to_v xs) = EVERY no_Eval_v xs
 Proof
   Induct
-  \\ simp [list_to_v_def, no_Eval_v_cases]
+  \\ simp [list_to_v_def]
 QED
 
 Theorem no_Eval_v_v_to_list:
   !v xs. v_to_list v = SOME xs /\ no_Eval_v v ==> EVERY no_Eval_v xs
 Proof
   recInduct terminationTheory.v_to_list_ind
-  \\ rw [terminationTheory.v_to_list_def, no_Eval_v_cases]
-  \\ fs [no_Eval_v_cases, option_case_eq]
+  \\ rw [terminationTheory.v_to_list_def]
+  \\ fs [option_case_eq]
   \\ rveq \\ fs []
 QED
 
@@ -267,14 +195,14 @@ Proof
   PairCases_on `r`
   \\ rw [do_app_cases, Boolv_def, ffiTheory.ffi_result_case_eq]
   \\ rw []
-  \\ fs [no_Eval_v_cases, div_exn_v_def, sub_exn_v_def, chr_exn_v_def]
+  \\ fs [div_exn_v_def, sub_exn_v_def, chr_exn_v_def]
   \\ fs [store_assign_def, store_alloc_def] \\ rveq \\ fs []
   \\ TRY (irule IMP_EVERY_LUPDATE)
-  \\ simp [no_Eval_v_list_to_v, EVERY_MAP, no_Eval_v_cases]
+  \\ simp [no_Eval_v_list_to_v, EVERY_MAP]
   \\ imp_res_tac no_Eval_v_v_to_list
   \\ fs [option_case_eq] \\ rveq \\ fs []
   \\ TRY (irule IMP_EVERY_LUPDATE)
-  \\ simp [no_Eval_v_cases]
+  \\ simp []
   \\ TRY (
     CHANGED_TAC (fs [store_lookup_def])
     \\ imp_res_tac EVERY_EL
@@ -307,7 +235,7 @@ Proof
   \\ fs [option_case_eq, pair_case_eq, bool_case_eq, store_v_case_eq,
         match_result_case_eq]
   \\ rveq \\ fs []
-  \\ fs [Q.ISPEC `Match b` EQ_SYM_EQ, no_Eval_v_cases]
+  \\ fs [Q.ISPEC `Match b` EQ_SYM_EQ]
   \\ TRY (
     CHANGED_TAC (fs [store_lookup_def])
     \\ imp_res_tac EVERY_EL
@@ -333,10 +261,12 @@ Triviality nsSing_eq_bind = namespaceTheory.nsSing_def
   |> REWRITE_RULE [GSYM namespaceTheory.nsBind_def,
     GSYM namespaceTheory.nsEmpty_def]
 
-Definition not_oracle_def[simp]:
+Definition not_oracle_def:
   not_oracle (SOME (EvalOracle _)) = F /\
   not_oracle _ = T
 End
+
+val _ = bossLib.augment_srw_ss [rewrites [not_oracle_def]];
 
 Triviality pair_CASE_eq_pairarg:
   pair_CASE p f = (\(x, y). f x y) p
@@ -349,6 +279,8 @@ Theorem combine_dec_result_eq_Rerr:
 Proof
   Cases_on `r` \\ simp [combine_dec_result_def]
 QED
+
+val s = mk_var ("s", ``: 'ffi semanticPrimitives$state``);
 
 Theorem no_Eval_evaluate:
   (! ^s env exps s' res.
@@ -408,60 +340,793 @@ Proof
      super tedious to go through 20-plus cases for this *)
   ho_match_mp_tac terminationTheory.full_evaluate_ind
   \\ rw [terminationTheory.full_evaluate_def]
-  \\ fs [has_Eval_def, has_Eval_dec_def, EVERY_REVERSE, no_Eval_v_cases]
+  \\ fs [has_Eval_def, has_Eval_dec_def, EVERY_REVERSE]
   \\ rveq \\ fs []
   \\ fs [pair_case_eq, result_case_eq, error_result_case_eq, bool_case_eq,
-    option_case_eq, exp_or_val_case_eq]
+    option_case_eq, exp_or_val_case_eq, match_result_case_eq,
+    eval_state_case_eq,
+    do_log_def, do_if_def, build_conv_def, dec_clock_def, declare_env_def,
+    bind_exn_v_def]
   \\ rw []
   \\ fs [pair_CASE_eq_pairarg, combine_dec_result_eq_Rerr]
   \\ rpt (pairarg_tac \\ fs [])
-  \\ rveq \\ fs []
-  \\ fs [match_result_case_eq, do_log_def, do_if_def, build_conv_def,
-        bind_exn_v_def, bool_case_eq, pair_case_eq]
   \\ ntac 2 (rveq \\ fs [])
-  \\ TRY (drule do_opapp_no_Eval)
-  \\ TRY (drule do_app_no_Eval)
-  \\ fs [Q.ISPEC `(a, b)` EQ_SYM_EQ, no_Eval_v_cases, EVERY_REVERSE]
-  \\ imp_res_tac evaluate_sing
-  \\ TRY (drule_then imp_res_tac (CONJUNCT1 pmatch_no_Eval))
-  \\ TRY (CHANGED_TAC (simp [combine_dec_result_def]) \\ CASE_TAC \\ fs [])
-  \\ TRY (qpat_x_assum `no_Eval_env _ ==> _` mp_tac \\ impl_tac)
-  \\ simp [EVERY_REVERSE]
-  \\ rpt disch_tac
-  \\ ntac 2 (rveq \\ fs [])
-  \\ fs [dec_clock_def, build_rec_env_merge, nsAppend_to_nsBindList,
-    declare_env_def, option_case_eq, eval_state_case_eq, pair_case_eq]
-  \\ rveq \\ fs []
   \\ rfs []
-  \\ simp [list_result_def]
+  \\ imp_res_tac evaluate_sing
+  \\ rveq \\ fs []
+  \\ fs [Q.ISPEC `(a, b)` EQ_SYM_EQ, EVERY_REVERSE]
+  \\ rfs []
+  \\ TRY (MAP_FIRST (drule_then strip_assume_tac) [
+    do_opapp_no_Eval, do_app_no_Eval, CONJUNCT1 pmatch_no_Eval])
+  \\ rfs [EVERY_REVERSE]
+  \\ TRY (qpat_x_assum `_ ==> _` mp_tac
+    \\ (impl_tac THENL [rpt strip_tac, strip_tac])
+    \\ fs [] \\ rfs [])
+  \\ rveq \\ fs []
+  \\ simp [namespaceTheory.nsOptBind_def, build_rec_env_merge,
+        nsAppend_to_nsBindList, combine_dec_result_def, no_Eval_extend,
+        combine_dec_result_def,
+        GSYM (SIMP_RULE (srw_ss ()) [] extend_dec_env_def)]
+  \\ rpt CASE_TAC
+  \\ fs [alist_to_ns_to_bind2, nsSing_eq_bind]
   \\ TRY (
-    CHANGED_TAC (simp [namespaceTheory.nsOptBind_def]) \\ CASE_TAC
-    \\ simp []
-  )
-  \\ TRY (
-    simp [no_Eval_env_def, alist_to_ns_to_bind2, nsSing_eq_bind]
-    \\ MAP_FIRST irule [env_rel_add_nsBind, env_rel_add_nsBindList, env_rel_nsLift]
+    simp [no_Eval_env_def]
+    \\ MAP_FIRST irule [env_rel_add_nsBind, env_rel_add_nsBindList,
+        env_rel_nsLift]
     \\ simp [GSYM no_Eval_env_def]
   )
-  \\ simp [Q.SPEC `x with <| v := nsEmpty |>` no_Eval_env_def,
-        Q.SPECL [`R`, `x with <| v := nsEmpty |>`] env_rel_def]
+  \\ simp [Q.SPEC `x with <| v := nsEmpty |>` no_Eval_env_def, env_rel_nsEmpty,
+    no_Eval_extend]
   \\ TRY (
     irule EVERY2_refl
     \\ fs [GSYM EVERY_MEM, EVERY_MAP]
     \\ first_assum (fn t => mp_tac t \\ match_mp_tac EVERY_MONOTONIC)
-    \\ simp [FORALL_PROD, quotient_pairTheory.PAIR_REL_THM, no_Eval_v_cases,
-        EVERY_MAP]
+    \\ simp [FORALL_PROD, quotient_pairTheory.PAIR_REL_THM, EVERY_MAP]
   )
-  \\ rfs [no_Eval_extend, combine_dec_result_def]
-  \\ fs [no_Eval_extend, GSYM (SIMP_RULE (srw_ss ()) [] extend_dec_env_def)]
-  \\ rveq \\ fs []
-  \\ simp [no_Eval_v_cases, EVERY_REVERSE]
-  \\ TRY (qpat_x_assum `_ <> Rerr _ ==> _` mp_tac \\ impl_tac \\ strip_tac)
-  \\ rveq \\ fs []
-  \\ TRY (fs [no_Eval_env_def, env_rel_def] \\ res_tac
-    \\ fs [no_Eval_v_rel_rules] \\ NO_TAC)
+  \\ TRY (fs [no_Eval_env_def, env_rel_def] \\ res_tac \\ fs [] \\ NO_TAC)
 QED
 
+(* the Eval case. adding the compiler adjusts the code, adds a
+   compiler state to the refs, and adjusts every Env to contain
+   the new module.
+*)
+
+Theorem namespace1_size:
+  namespace1_size f1 f2 f3 xs =
+    LENGTH xs + SUM (MAP (namespace2_size f1 f2 f3) xs)
+Proof
+  Induct_on `xs` \\ simp [namespaceTheory.namespace_size_def]
+QED
+
+Definition nsAdj_def:
+  nsAdj (Bind nms mods) = Bind nms
+        (MAP (\(nm, m). (adj_mod_name nm, nsAdj m)) mods)
+Termination
+  WF_REL_TAC `measure (namespace_size (K 0) (K 0) (K 0))`
+  \\ rw [namespaceTheory.namespace_size_def]
+  \\ fs [MEM_SPLIT, namespace1_size, namespaceTheory.namespace_size_def,
+    SUM_APPEND]
+End
+
+Definition env_adj_rel_def:
+  env_adj_rel v_rel (env : v sem_env) env' <=>
+    nsDomMod env'.c DIFF IMAGE (CONS compiler_module_name) UNIV =
+        IMAGE (MAP adj_mod_name) (nsDomMod env.c) /\
+    nsDom env'.c DIFF IMAGE (Long compiler_module_name) UNIV =
+        IMAGE adj_id (nsDom env.c) /\
+    nsDomMod env'.v DIFF IMAGE (CONS compiler_module_name) UNIV =
+        IMAGE (MAP adj_mod_name) (nsDomMod env.v) /\
+    nsDom env'.v DIFF IMAGE (Long compiler_module_name) UNIV =
+        IMAGE adj_id (nsDom env.v) /\
+    (!nm x. nsLookup env.c nm = SOME x ==>
+        nsLookup env'.c (adj_id nm) = SOME x) /\
+    (!nm x y. nsLookup env.v nm = SOME x /\
+        nsLookup env'.v (adj_id nm) = SOME y ==>
+        v_rel x y)
+End
+
+Theorem env_adj_rel_mono_rel:
+  (!y z. R y z ==> R' y z) ==>
+  env_adj_rel R env env' ==>
+  env_adj_rel R' env env'
+Proof
+  simp [env_adj_rel_def] \\ metis_tac []
+QED
+
+val _ = IndDefLib.add_mono_thm env_adj_rel_mono_rel;
+
+Theorem env_adj_rel_nsLookup_c:
+  env_adj_rel R env env' /\
+  nsLookup env.c id = SOME data ==>
+  nsLookup env'.c (adj_id id) = SOME data
+Proof
+  rw [env_adj_rel_def]
+QED
+
+Theorem adj_mod_name_not_compiler:
+  adj_mod_name m ≠ compiler_module_name
+Proof
+  rw [adj_mod_name_def]
+  \\ strip_tac
+  \\ fs []
+  \\ fs [stringTheory.isPREFIX_STRCAT]
+  \\ rveq \\ fs []
+QED
+
+Theorem adj_id_not_compiler:
+  !id x. adj_id id ≠ Long compiler_module_name x
+Proof
+  Induct
+  \\ simp [adj_id_def, adj_mod_name_not_compiler]
+QED
+
+Theorem adj_mod_name_11:
+  (adj_mod_name m = adj_mod_name m') = (m = m')
+Proof
+  rw [adj_mod_name_def]
+  \\ EQ_TAC
+  \\ rw []
+  \\ TRY strip_tac
+  \\ fs []
+  \\ first_x_assum (fn t => mp_tac t \\ simp [] \\ irule IS_PREFIX_TRANS)
+  \\ goal_assum (first_x_assum o mp_then Any mp_tac)
+  \\ simp []
+QED
+
+Theorem adj_id_11:
+  !id id'. (adj_id id = adj_id id') = (id = id')
+Proof
+  Induct \\ simp [adj_id_def]
+  \\ gen_tac \\ Cases
+  \\ simp [adj_id_def, adj_mod_name_11]
+QED
+
+Triviality env_adj_rel_nsLookup_helper:
+  m = IMAGE f (nsDom ns) /\ nsLookup ns id = SOME v ==>
+  f id ∈ m
+Proof
+  rw [nsLookup_nsDom]
+  \\ simp []
+  \\ metis_tac []
+QED
+
+Theorem env_adj_rel_nsLookup_v:
+  env_adj_rel R env env' /\
+  nsLookup env.v id = SOME v ==>
+  ?v'. nsLookup env'.v (adj_id id) = SOME v' /\ R v v'
+Proof
+  rw [env_adj_rel_def]
+  \\ drule_then drule env_adj_rel_nsLookup_helper
+  \\ simp [adj_id_not_compiler, nsLookup_nsDom]
+  \\ rw []
+  \\ fs []
+  \\ res_tac
+QED
+
+Theorem env_adj_rel_nsBind:
+  R v v' /\ env_adj_rel R (env with v := vs) (env' with v := vs') ==>
+  env_adj_rel R (env with v := nsBind nm v vs) (env' with v := nsBind nm v' vs')
+Proof
+  rw [env_adj_rel_def, adj_id_def]
+  \\ Cases_on `nm'` \\ fs [adj_id_def]
+  >- (
+    Cases_on `nm = n` \\ fs [nsLookup_nsBind]
+    \\ res_tac
+    \\ rfs [adj_id_def]
+  )
+  \\ res_tac
+  \\ rfs [adj_id_def]
+QED
+
+Theorem env_adj_rel_nsBindList:
+  !xs ys. env_adj_rel R (env with v := ev) (env' with v := ev') /\
+  LIST_REL ((=) ### R) xs ys ==>
+  env_adj_rel R (env with v := nsBindList xs ev)
+    (env' with v := nsBindList ys ev')
+Proof
+  Induct
+  \\ simp [FORALL_PROD, EXISTS_PROD]
+  \\ rw []
+  \\ fs [namespaceTheory.nsBindList_def, quotient_pairTheory.PAIR_REL_THM]
+  \\ irule env_adj_rel_nsBind
+  \\ simp []
+QED
+
+
+Inductive v_rel:
+  (!id env'. v_to_env_id v = SOME id /\ lookup_env es id = SOME env' /\
+        env_adj_rel (v_rel es) env env' ==>
+    v_rel es (Env env) v) /\
+  (LIST_REL (v_rel es) xs ys ==>
+    v_rel es (Vectorv xs) (Vectorv ys)) /\
+  (LIST_REL (v_rel es) xs ys ==>
+    v_rel es (Conv stmp xs) (Conv stmp ys)) /\
+  (env_adj_rel (v_rel es) env env' ==>
+    v_rel es (Closure env nm x) (Closure env' nm (compile_exp x))) /\
+  (env_adj_rel (v_rel es) env env' ==>
+    v_rel es (Recclosure env funs nm)
+        (Recclosure env' (MAP (I ## I ## compile_exp) funs) nm)) /\
+  (v_rel es (Litv l) (Litv l)) /\
+  (v_rel es (Loc n) (Loc (n + 1)))
+End
+
+Theorem v_rel_l_simps =
+  [``v_rel es (Litv l) v``, ``v_rel es (Conv cn vs) v``,
+    ``v_rel es (Loc l) v``, ``v_rel es (Vectorv vs) v``,
+    ``v_rel es (Env e) v``, ``v_rel es (Recclosure env funs nm) v``,
+    ``v_rel es (Closure env nm x) v``]
+  |> map (SIMP_CONV (srw_ss ()) [Once v_rel_cases])
+  |> map GEN_ALL
+  |> LIST_CONJ
+
+val _ = bossLib.augment_srw_ss [rewrites [v_rel_l_simps]];
+
+Theorem v_rel_Boolv:
+  v_rel es (Boolv b) v = (v = Boolv b)
+Proof
+  rw [Boolv_def]
+QED
+
+val _ = bossLib.augment_srw_ss [rewrites [v_rel_Boolv]];
+
+Definition s_rel_def:
+  s_rel s s' <=>
+  ?es cs refs'. s' = s with <| refs := Refv cs :: refs';
+    eval_state := SOME (EvalOracle es) |> /\
+  LIST_REL (sv_rel (v_rel es)) s.refs refs' /\
+  s.eval_state = SOME EvalDecs /\
+  es.custom_do_eval = SOME do_eval_record /\
+  es.generation < LENGTH es.envs
+End
+
+Definition orac_s_def:
+  orac_s (SOME (EvalOracle es)) = es /\
+  orac_s _ = ARB "not EvalOracle"
+End
+
+val _ = bossLib.augment_srw_ss [rewrites [orac_s_def]];
+
+Definition es_forward_def:
+  es_forward es es' <=>
+  (es.custom_do_eval = SOME do_eval_record ==>
+    es'.custom_do_eval = SOME do_eval_record) /\
+  (LENGTH es.envs <= LENGTH es'.envs) /\
+  (!env_id env. lookup_env es env_id = SOME env ==>
+    lookup_env es' env_id = SOME env)
+End
+
+Theorem es_forward_refl:
+  es_forward es es
+Proof
+  simp [es_forward_def]
+QED
+
+Theorem es_forward_trans:
+  es_forward es es' /\ es_forward es' es'' ==>
+  es_forward es es''
+Proof
+  fs [es_forward_def]
+QED
+
+Theorem v_rel_forward:
+  !x y. v_rel es x y ==> es_forward es es' ==> v_rel es' x y
+Proof
+  ho_match_mp_tac v_rel_ind
+  \\ rw []
+  \\ full_simp_tac (bool_ss ++ ETA_ss) []
+  \\ fs [es_forward_def]
+  \\ res_tac
+  \\ simp []
+QED
+
+Theorem forward_rules:
+  (v_rel es x y /\ es_forward es es' ==> v_rel es' x y) /\
+  (LIST_REL (v_rel es) xs ys /\ es_forward es es' ==>
+    LIST_REL (v_rel es') xs ys) /\
+  (env_adj_rel (v_rel es) env env' /\ es_forward es es' ==>
+    env_adj_rel (v_rel es') env env') /\
+  (!xs ys. LIST_REL (sv_rel (v_rel es)) xs ys /\ es_forward es es' ==>
+    LIST_REL (sv_rel (v_rel es')) xs ys)
+Proof
+  rw []
+  \\ TRY (first_x_assum (fn t => mp_tac t \\ match_mp_tac LIST_REL_mono))
+  \\ rw []
+  \\ TRY (first_x_assum (fn t => mp_tac t \\ match_mp_tac sv_rel_mono))
+  \\ TRY (first_x_assum (fn t => mp_tac t \\ match_mp_tac env_adj_rel_mono_rel))
+  \\ rw []
+  \\ imp_res_tac v_rel_forward
+QED
+
+Definition match_result_rel_def:
+  match_result_rel nerr R mr1 mr2 <=> (case mr1 of
+    | No_match => mr2 = No_match
+    | Match_type_error => nerr \/ mr2 = Match_type_error
+    | Match x => ?y. mr2 = Match y /\ R x y)
+End
+
+Theorem store_lookup_rel:
+  LIST_REL (sv_rel R) refs refs' ==>
+  OPTREL (sv_rel R) (store_lookup i refs) (store_lookup i refs')
+Proof
+  rw [store_lookup_def, LIST_REL_EL_EQN]
+  \\ simp [OPTREL_def]
+QED
+
+Theorem s_rel_store_lookup:
+  s_rel s t /\ j = i + 1 /\ es = orac_s t.eval_state ==>
+  OPTREL (sv_rel (v_rel es)) (store_lookup i s.refs) (store_lookup j t.refs)
+Proof
+  rw [s_rel_def]
+  \\ drule store_lookup_rel
+  \\ simp [store_lookup_def, ADD1, EL_CONS]
+  \\ simp [GSYM ADD1]
+QED
+
+Theorem pmatch:
+  s_rel s t /\ es = orac_s t.eval_state /\ env_adj_rel (v_rel es) env env' ==>
+  (!env_c s_refs p x binds y binds'.
+  s_refs = s.refs /\ env_c = env.c /\
+  v_rel es x y /\
+  LIST_REL ((=) ### v_rel es) binds binds' ==>
+  match_result_rel T (LIST_REL ((=) ### v_rel es))
+    (pmatch env_c s_refs p x binds)
+    (pmatch env'.c t.refs (compile_pat p) y binds')
+  ) /\
+  (!env_c s_refs ps xs binds ys binds'.
+  s_refs = s.refs /\ env_c = env.c /\
+  LIST_REL (v_rel es) xs ys /\
+  LIST_REL ((=) ### v_rel es) binds binds' ==>
+  match_result_rel T (LIST_REL ((=) ### v_rel es))
+    (pmatch_list env_c s_refs ps xs binds)
+    (pmatch_list env'.c t.refs (MAP compile_pat ps) ys binds')
+  )
+Proof
+  disch_tac
+  \\ ho_match_mp_tac terminationTheory.pmatch_ind
+  \\ rw [terminationTheory.pmatch_def, match_result_rel_def,
+    quotient_pairTheory.PAIR_REL_THM, compile_pat_def]
+  \\ rveq \\ fs []
+  \\ fs [v_to_env_id_def, CaseEq "v", list_case_eq, option_case_eq]
+  \\ fs [terminationTheory.pmatch_def]
+  \\ imp_res_tac LIST_REL_LENGTH
+  \\ fs [ETA_THM]
+  >- (
+    TOP_CASE_TAC \\ fs []
+    \\ fs [option_case_eq, pair_case_eq, bool_case_eq]
+    \\ rveq \\ fs []
+    \\ every_case_tac
+    \\ fs []
+    \\ imp_res_tac env_adj_rel_nsLookup_c
+    \\ fs []
+    \\ res_tac
+    \\ fs []
+  )
+  >- (
+    drule s_rel_store_lookup
+    \\ simp []
+    \\ disch_then (qspec_then `lnum` mp_tac)
+    \\ every_case_tac \\ fs []
+    \\ rw [OPTREL_SOME, sv_rel_cases]
+    \\ fs []
+  )
+  >- (
+    first_x_assum (drule_then drule)
+    \\ every_case_tac \\ fs []
+    \\ first_x_assum (drule_then drule)
+    \\ simp []
+  )
+QED
+
+Triviality pmatch_use = UNDISCH_ALL pmatch |> CONJUNCT1 |> SPEC_ALL
+  |> Q.INST [`binds` |-> `[]`]
+  |> DISCH_ALL |> GEN_ALL
+  |> SIMP_RULE list_ss []
+
+Theorem can_pmatch_all:
+  can_pmatch_all env.c s.refs pats x /\
+  s_rel s t /\
+  env_adj_rel (v_rel (orac_s t.eval_state)) env env' /\
+  v_rel (orac_s t.eval_state) x y ==>
+  can_pmatch_all env'.c t.refs (MAP compile_pat pats) y
+Proof
+  rw []
+  \\ Induct_on `pats`
+  \\ rw [can_pmatch_all_def]
+  \\ drule pmatch_use
+  \\ rpt (disch_then drule)
+  \\ disch_then (qspec_then `h` mp_tac)
+  \\ simp [match_result_rel_def]
+  \\ every_case_tac
+  \\ fs []
+  \\ rw []
+  \\ simp []
+QED
+
+Theorem do_eq:
+  (! x y x' y' b. do_eq x y = Eq_val b /\
+  v_rel es x x' /\
+  v_rel es y y' ==>
+  do_eq x' y' = Eq_val b) /\
+  (! xs ys xs' ys' b. do_eq_list xs ys = Eq_val b /\
+  LIST_REL (v_rel es) xs xs' /\
+  LIST_REL (v_rel es) ys ys' ==>
+  do_eq_list xs' ys' = Eq_val b)
+Proof
+  ho_match_mp_tac do_eq_ind
+  \\ rw [do_eq_def]
+  \\ rw [do_eq_def]
+  \\ imp_res_tac LIST_REL_LENGTH
+  \\ rveq \\ fs []
+  \\ fs [eq_result_case_eq, bool_case_eq]
+  \\ fs []
+QED
+
+Theorem store_assign:
+  store_assign lnum sv refs = SOME refs2 /\
+  LIST_REL (sv_rel R) refs refs3 /\
+  sv_rel R sv sv' ==>
+  ?refs4.
+  LIST_REL (sv_rel R) refs2 refs4 /\
+  (!sv1.  store_assign (lnum + 1) sv' (sv1 :: refs3) = SOME (sv1 :: refs4))
+Proof
+  rw [store_assign_def, ADD1, EL_CONS]
+  \\ simp [GSYM ADD1, LUPDATE_def]
+  \\ imp_res_tac LIST_REL_LENGTH
+  \\ fs [EVERY2_LUPDATE_same]
+  \\ fs [LIST_REL_EL_EQN]
+  \\ res_tac
+  \\ fs [sv_rel_cases, store_v_same_type_def] \\ rveq \\ fs []
+QED
+
+Theorem store_lookup:
+  LIST_REL (sv_rel R) refs refs' /\
+  store_lookup n refs = SOME sv ==>
+  ?sv'. sv_rel R sv sv' /\
+  (!sv1. store_lookup (n + 1) (sv1 :: refs') = SOME sv')
+Proof
+  rw [store_lookup_def, LIST_REL_EL_EQN, GSYM ADD1]
+  \\ res_tac
+QED
+
+Theorem sv_rel_l_cases =
+  [``sv_rel R (Refv rv) v``, ``sv_rel R (W8array xs) v``,
+        ``sv_rel R (Varray vs) v``]
+  |> map (SIMP_CONV (srw_ss ()) [sv_rel_cases])
+  |> map GEN_ALL |> LIST_CONJ
+
+Theorem do_app:
+  do_app (s.refs, s.ffi) op (REVERSE xs) = SOME ((refs, ffi), r) /\
+  s_rel s t /\
+  LIST_REL (v_rel (orac_s t.eval_state)) xs ys /\
+  r <> Rerr (Rabort Rtype_error)
+  ==>
+  ? ref1 refs' r' es.
+  es = orac_s t.eval_state /\
+  do_app (t.refs, t.ffi) op (REVERSE ys) = SOME ((ref1 :: refs', ffi), r') /\
+  ref1 = HD t.refs /\
+  LIST_REL (sv_rel (v_rel es)) refs refs' /\
+  result_rel (v_rel es) (v_rel es) r r'
+
+Proof
+
+  rw [s_rel_def]
+  \\ fs []
+  \\ last_x_assum mp_tac
+  \\ simp [Once do_app_cases] \\ rw [listTheory.SWAP_REVERSE_SYM]
+  \\ fs [CaseEq "ffi_result", option_case_eq] \\ rveq \\ fs []
+  \\ simp [do_app_def]
+  \\ simp [div_exn_v_def, sub_exn_v_def, chr_exn_v_def,
+        EVERY2_refl, MEM_MAP, PULL_EXISTS]
+  \\ TRY (drule_then imp_res_tac (CONJUNCT1 do_eq))
+  \\ TRY (drule_then imp_res_tac store_lookup)
+  \\ TRY (drule_then drule store_assign
+        \\ simp [sv_rel_l_cases, PULL_EXISTS]
+        \\ disch_then drule)
+
+  \\ rw []
+  \\ rw []
+  \\ imp_res_tac LIST_REL_LENGTH
+  \\ fs [PULL_EXISTS, store_alloc_def, sv_rel_l_cases, ADD1]
+  \\ rveq \\ fs []
+
+  \\ TRY (drule_then drule store_assign
+        \\ simp [sv_rel_l_cases, PULL_EXISTS]
+        \\ disch_then drule)
+
+
+  \\ TRY (drule_then imp_res_tac v_to_char_list1)
+  \\ TRY (drule_then kall_tac v_to_list1 \\ imp_res_tac v_to_list1)
+  \\ TRY (drule_then kall_tac store_lookup \\ imp_res_tac store_lookup)
+  \\ TRY (irule EVERY2_refl)
+  \\ simp [v_rel1_l_cases, v_rel1_Boolv, v_rel1_list_to_v, LIST_REL_APPEND_EQ]
+
+  \\ fs [PULL_EXISTS, store_alloc_def, sv_rel_l_cases]
+  \\ rveq \\ fs []
+  \\ simp [ADD1]
+
+  \\ insts_tac
+  \\ TRY (drule_then imp_res_tac vs_to_string1)
+  \\ rveq \\ fs []
+  \\ imp_res_tac LIST_REL_LENGTH
+  \\ rveq \\ fs []
+  \\ fs [LIST_REL_REPLICATE_same]
+  \\ TRY (fs [LIST_REL_EL_EQN] \\ NO_TAC)
+
+
+(* well, we were doing so well here .. sort of
+
+  EnvLookup puts us in a world of difficulties
+
+
+Theorem pairarg_to_pair_map:
+  (\(x, y). (f x, g y)) = (f ## g)
+Proof
+  simp [FUN_EQ_THM, FORALL_PROD]
+QED
+
+Theorem s_rel_clock:
+  s_rel s t ==> s.clock = t.clock /\
+    s_rel (dec_clock s) (dec_clock t)
+Proof
+  rw [s_rel_def]
+  \\ fs [evaluateTheory.dec_clock_def]
+  \\ simp [semanticPrimitivesTheory.state_component_equality]
+QED
+
+
+Theorem compile_correct:
+
+  (! ^s env exps s' res es t env'.
+  evaluate s env exps = (s', res) /\
+  s_rel s t /\
+  env_adj_rel (v_rel (orac_s t.eval_state)) env env' /\
+  res <> Rerr (Rabort Rtype_error) ==>
+  ? es' t' res'.
+  evaluate t env' (MAP compile_exp exps) = (t', res') /\
+  s_rel s' t' /\
+  es' = orac_s t'.eval_state /\
+  result_rel (LIST_REL (v_rel es')) (v_rel es') res res' /\
+  es_forward (orac_s t.eval_state) es')
+  /\
+  (! ^s env x pes err_x s' res es t env' y err_y.
+  evaluate_match s env x pes err_x = (s', res) /\
+  s_rel s t /\
+  es = orac_s t.eval_state /\
+  env_adj_rel (v_rel es) env env' /\
+  v_rel es x y /\
+  v_rel es err_x err_y /\
+  res <> Rerr (Rabort Rtype_error) ==>
+  ?es' t' res'.
+  evaluate_match t env' y (MAP (compile_pat ## compile_exp) pes) err_y =
+    (t', res') /\
+  s_rel s' t' /\
+  es' = orac_s t'.eval_state /\
+  result_rel (LIST_REL (v_rel es')) (v_rel es') res res' /\
+  es_forward es es')
+  /\
+  (! ^s env decs s' res t env'.
+  evaluate_decs s env decs = (s', res) /\
+  s_rel s t /\
+  env_adj_rel (v_rel (orac_s t.eval_state)) env env' /\
+  res <> Rerr (Rabort Rtype_error) ==>
+  ?es' t' res'.
+  evaluate_decs t env' (MAP compile_dec decs) = (t', res') /\
+  s_rel s' t' /\
+  es' = orac_s t'.eval_state /\
+  result_rel (env_adj_rel (v_rel es')) (v_rel es') res res' /\
+  es_forward (orac_s t.eval_state) es')
+
+Proof
+
+  ho_match_mp_tac terminationTheory.full_evaluate_ind
+  \\ rpt conj_tac
+  \\ rpt (gen_tac ORELSE disch_tac)
+  \\ fs [compile_exp_def, terminationTheory.full_evaluate_def]
+  \\ rveq \\ fs []
+
+  >- (
+    insts_tac
+  )
+
+  >- (
+    eval_cases_tac
+    \\ insts_tac
+  )
+
+  >- (
+    insts_tac
+  )
+
+  >- (
+    eval_cases_tac
+    \\ insts_tac
+  )
+
+  >- (
+    eval_cases_tac
+    \\ insts_tac
+    \\ drule_then assume_tac can_pmatch_all
+    \\ insts_tac
+    \\ fs [MAP_MAP_o, pairarg_to_pair_map, miscTheory.o_PAIR_MAP]
+    \\ insts_tac
+  )
+
+  >- (
+    eval_cases_tac
+    \\ fs [ETA_THM, MAP_REVERSE]
+    \\ insts_tac
+    \\ fs [do_con_check_def, build_conv_def]
+    \\ every_case_tac \\ fs [] \\ rveq \\ fs []
+    \\ drule_then drule env_adj_rel_nsLookup_c
+    \\ simp []
+  )
+
+  >- (
+    eval_cases_tac
+    \\ drule_then drule env_adj_rel_nsLookup_v
+    \\ rw []
+    \\ simp []
+    \\ insts_tac
+  )
+
+  >- (
+    insts_tac
+  )
+
+  >- (
+    (* App *)
+
+    reverse (fs [pair_case_eq, result_case_eq] \\ rveq \\ fs [])
+    >- (
+      fs [MAP_REVERSE, ETA_THM]
+      \\ rw [terminationTheory.evaluate_def, do_con_check_def]
+      \\ insts_tac
+    )
+    \\ insts_tac
+    \\ Cases_on `op = Opapp`
+
+    >- (
+
+      rveq \\ fs []
+      \\ fs [ETA_THM, MAP_REVERSE, terminationTheory.evaluate_def]
+      \\ imp_res_tac s_rel_clock
+      \\ fs [do_opapp_def]
+      \\ eval_cases_tac
+      \\ fs [listTheory.SWAP_REVERSE_SYM, CaseEq "v"] \\ rveq \\ fs []
+      \\ fs [listTheory.SWAP_REVERSE, miscTheory.FST_triple]
+      \\ fs [find_recfun_ALOOKUP]
+      \\ eval_cases_tac
+      \\ insts_tac
+      \\ TRY (drule (Q.ISPECL [`I ## compile_exp`, `I`]
+        (GEN_ALL ALOOKUP_MAP_FST_INJ_SOME)))
+      \\ simp []
+      \\ rfs [EVAL ``(dec_clock s).eval_state``]
+      \\ first_x_assum (q_pmatch_then `evaluate _ _ _` mp_tac)
+      \\ impl_tac \\ rw [] \\ insts_tac
+      \\ irule env_adj_rel_nsBind
+      \\ insts_tac
+      \\ simp [build_rec_env_merge, nsAppend_to_nsBindList]
+      \\ irule env_adj_rel_nsBindList
+      \\ simp [LIST_REL_MAP1, SIMP_RULE (bool_ss ++ ETA_ss) [] LIST_REL_MAP2]
+      \\ simp [ELIM_UNCURRY, quotient_pairTheory.PAIR_REL_THM, EVERY2_refl]
+    )
+
+    \\ Cases_on `op = Eval`
+    >- (
+      fs [do_eval_res_def, terminationTheory.evaluate_def, do_con_check_def]
+      \\ simp [MAP_REVERSE, ETA_THM, build_conv_def]
+      \\ eval_cases_tac
+      \\ insts_tac
+
+      \\ cheat
+    )
+    \\ eval_cases_tac
+    \\ simp [MAP_REVERSE, ETA_THM, terminationTheory.evaluate_def]
+
+
+
+    eval_cases_tac
+    \\ fs [ETA_THM]
+    \\ insts_tac
+
+    \\ first_x_assum (do_match_inst ``s_rel`` ["m", "i"])
+    \\ rfs []
+    \\ first_x_assum (do_match_inst ``env_rel`` ["_", "m", "i"])
+    \\ rveq \\ fs []
+    \\ TRY (qpat_x_assum `_ ==> _` mp_tac
+      \\ (impl_tac THENL [rpt strip_tac, strip_tac]))
+ 
+    \\ fsrw_tac [SATISFY_ss] [forward_rules]
+    \\ fs []
+
+
+fun do_match_inst const data cont thm = let
+    val (vs, t1) = strip_forall (concl thm)
+    val (lhs, _) = dest_imp t1
+    val vset = HOLset.addList (empty_tmset, vs)
+    val mem_vset = curry HOLset.member vset
+    fun match_vars_free ("m", t) = all (not o mem_vset) (free_vars t)
+      | match_vars_free _ = true
+    fun inst_var ("i", t) = exists mem_vset (free_vars t)
+      | inst_var _ = false
+    val prems = strip_conj lhs
+      |> filter (same_const const o fst o strip_comb)
+      |> filter (all match_vars_free o zip data o snd o strip_comb)
+      |> filter (exists inst_var o zip data o snd o strip_comb)
+  in MAP_FIRST (fn prem => let
+    val const = strip_comb prem |> fst
+    val prem_els = strip_comb prem |> snd |> zip data
+    fun matches (("m", t), t') = term_eq t t'
+      | matches _ = true
+    fun assum_match a = case strip_comb a of (c, xs) =>
+      term_eq c const andalso all matches (zip prem_els xs)
+  in FIRST_ASSUM (fn a => if assum_match (concl a)
+  then let
+    val fvs = FVL [concl thm, concl a] empty_tmset
+    val (vs2, sub) = quantHeuristicsTools.list_variant (HOLset.listItems fvs) vs
+    val thm2 = SPECL vs2 thm
+    val prem2 = subst sub prem
+    val els2 = strip_comb prem2 |> snd |> zip data
+    fun get_subst (("i", t), t') = fst (match_term t t')
+      | get_subst _ = []
+    val sub2 = strip_comb (concl a) |> snd |> zip els2
+      |> map get_subst |> List.concat
+    val thm3 = INST sub2 thm2
+    val fvs2 = FVL [concl thm3] empty_tmset
+    val vs3 = filter (curry HOLset.member fvs2) vs2
+    val thm4 = GENL vs3 thm3
+  in cont thm4 end
+  else NO_TAC)
+  end) prems
+  end
+
+fun do_inst const data = first_x_assum (do_match_inst const data mp_tac)
+  \\ simp [] \\ TRY disch_tac
+
+val find_toplevel_bool = let
+    fun find1 t = find_terms (fn t => type_of t = bool) t
+        |> filter (not o fast_term_eq t)
+    fun fvs t = FVL [t] empty_tmset
+    fun is_toplevel s t = HOLset.isSubset (fvs t, s)
+  in fn t => case find1 t of [] => []
+    | ts => filter (is_toplevel (fvs t)) ts
+  end
+
+fun propose_subgoal_tac1 pat (asms, goal) = 
+  (map find_toplevel_bool (goal :: asms)
+    |> List.concat
+    |> filter (can (match_term pat))
+    |> MAP_FIRST (reverse o suff_tac)) (asms, goal)
+
+fun propose_subgoal_tac pats = MAP_FIRST (Q_TAC propose_subgoal_tac1) pats
+
+
+
+val forward_tac = MAP_FIRST (drule_then irule)
+    (es_forward_trans :: IMP_CANON forward_rules)
+
+val insts_tac = rpt (FIRST ([
+      do_inst ``s_rel`` ["m", "i"],
+      do_inst ``env_adj_rel`` ["_", "m", "i"],
+      do_inst ``v_rel`` ["_", "m", "i"],
+      CHANGED_TAC (fs [Q.ISPEC `(a, b)` EQ_SYM_EQ, es_forward_refl] \\ rfs []),
+      forward_tac,
+      first_x_assum (fn t => mp_tac t \\ (impl_tac THENL
+            [rpt conj_tac \\ forward_tac, disch_tac])),
+      conj_tac \\ forward_tac
+(*
+      propose_subgoal_tac [`env_adj_rel _ _ _`, `v_rel _ _ _`]
+            THENL [forward_tac, disch_tac]
+*)
+    ] 
+    ))
+
+val eval_cases_tac =
+  fs [pair_case_eq, result_case_eq, error_result_case_eq, bool_case_eq,
+        option_case_eq, list_case_eq, exp_or_val_case_eq, match_result_case_eq]
+  \\ rveq \\ fs [] 
+  \\ imp_res_tac evaluate_sing
+  \\ rveq \\ fs [] 
 
 
 
