compiler/backend/source_evalScript.sml
@@ -116,27 +116,42 @@ Definition adj_id_def:
   adj_id (Long mnm id) = Long (adj_mod_name mnm) (adj_id id)
 End
 
+Definition compile_pat_def:
+  (compile_pat (Pcon id ps) = Pcon (OPTION_MAP adj_id id) (MAP compile_pat ps))
+  ∧
+  (compile_pat (Pref p) = Pref (compile_pat p)) ∧
+  (compile_pat (Ptannot p t) = compile_pat p) ∧
+  (compile_pat p = p)
+Termination
+  WF_REL_TAC `measure pat_size`
+  \\ simp_tac bool_ss [GSYM size_abbrevs, pats_size_thm]
+  \\ rw []
+  \\ fs [MEM_SPLIT, SUM_APPEND]
+End
+
 Definition compile_exp_def:
-  (compile_exp (Var id)) = Var (adj_id id) ∧
-  (compile_exp (Raise e)) = Raise (compile_exp e) ∧
-  (compile_exp (Handle e pes)) = Handle (compile_exp e)
-    (MAP (\(a, x). (a, compile_exp x)) pes) ∧
-  (compile_exp (Con cn es)) = Con cn (MAP compile_exp es) ∧
-  (compile_exp (Fun x e)) = Fun x (compile_exp e) ∧
-  (compile_exp (App op es)) = (if op = Eval
-    then App Opapp [Var (Long compiler_module_name (Short "eval")); Con NONE es]
-    else App op (MAP compile_exp es)) ∧
-  (compile_exp (Log lop e1 e2)) = Log lop (compile_exp e1) (compile_exp e2) ∧
-  (compile_exp (If e1 e2 e3)) =
-    If (compile_exp e1) (compile_exp e2) (compile_exp e3) ∧
-  (compile_exp (Mat e pes)) = Mat (compile_exp e)
-    (MAP (\(a, x). (a, compile_exp x)) pes) ∧
-  (compile_exp (Let nm e1 e2)) = Let nm (compile_exp e1) (compile_exp e2) ∧
-  (compile_exp (Letrec funs e)) = Letrec
+  (compile_exp (Var id) = Var (adj_id id)) ∧
+  (compile_exp (Raise e) = Raise (compile_exp e)) ∧
+  (compile_exp (Handle e pes) = Handle (compile_exp e)
+    (MAP (\(p, x). (compile_pat p, compile_exp x)) pes)) ∧
+  (compile_exp (Con cn es) = Con (OPTION_MAP adj_id cn) (MAP compile_exp es)) ∧
+  (compile_exp (Fun x e) = Fun x (compile_exp e)) ∧
+  (compile_exp (App op es) = (if op = Eval
+    then App Opapp [Var (Long compiler_module_name (Short "eval"));
+        Con NONE (MAP compile_exp es)]
+    else App op (MAP compile_exp es))) ∧
+  (compile_exp (Log lop e1 e2) = Log lop (compile_exp e1) (compile_exp e2)) ∧
+  (compile_exp (If e1 e2 e3) =
+    If (compile_exp e1) (compile_exp e2) (compile_exp e3)) ∧
+  (compile_exp (Mat e pes) = Mat (compile_exp e)
+    (MAP (\(p, x). (compile_pat p, compile_exp x)) pes)) ∧
+  (compile_exp (Let nm e1 e2) = Let nm (compile_exp e1) (compile_exp e2)) ∧
+  (compile_exp (Letrec funs e) = Letrec
     (MAP (\(a, b, x). (a, b, compile_exp x)) funs)
-    (compile_exp e) ∧
-  (compile_exp (Tannot x t) = Tannot (compile_exp x) t) ∧
-  (compile_exp (Lannot x locs) = Lannot (compile_exp x) locs)
+    (compile_exp e)) ∧
+  (compile_exp (Tannot x t) = compile_exp x) ∧
+  (compile_exp (Lannot x locs) = compile_exp x) ∧
+  (compile_exp exp = exp)
 Termination
   WF_REL_TAC `measure exp_size`
   \\ rw [exp_size_def]
@@ -146,13 +161,35 @@ Termination
   \\ fs [MEM_SPLIT, exp_size_def, SUM_APPEND]
 End
 
+Theorem ast_t1_size:
+  ast_t1_size ts = LENGTH ts + SUM (MAP ast_t_size ts)
+Proof
+  Induct_on `ts` \\ simp [ast_t_size_def]
+QED
+
+Definition compile_type_def:
+  (compile_type (Atapp ts id) = Atapp (MAP compile_type ts) (adj_id id)) /\
+  (compile_type (Attup ts) = Attup (MAP compile_type ts)) /\
+  (compile_type (Atfun t1 t2) = Atfun (compile_type t1) (compile_type t2)) /\
+  (compile_type t = t)
+Termination
+  WF_REL_TAC `measure ast_t_size`
+  \\ rw [ast_t_size_def, ast_t1_size]
+  \\ fs [MEM_SPLIT, ast_t_size_def, SUM_APPEND]
+End
+
 Definition compile_dec_def:
   (compile_dec (Dlet loc nm e) = Dlet loc nm (compile_exp e)) ∧
   (compile_dec (Dletrec locs funs) =
         Dletrec locs (MAP (\(a, b, x). (a, b, compile_exp x)) funs)) ∧
-  (compile_dec (Dmod mnm ds) = Dmod mnm (MAP compile_dec ds)) ∧
+  (compile_dec (Dmod mnm ds) = Dmod (adj_mod_name mnm) (MAP compile_dec ds)) ∧
   (compile_dec (Dlocal lds ds) = Dlocal (MAP compile_dec lds)
         (MAP compile_dec ds)) ∧
+  (compile_dec (Dexn locs cn ts) = Dexn locs cn (MAP compile_type ts)) ∧
+  (compile_dec (Dtabbrev locs vs nm t) =
+        Dtabbrev locs vs nm (compile_type t)) ∧
+  (compile_dec (Dtype locs td) = Dtype locs
+        (MAP (I ## (I ## MAP (I ## MAP compile_type))) td)) ∧
   (compile_dec d = d)
 Termination
   WF_REL_TAC `measure dec_size`
@@ -160,9 +197,94 @@ Termination
   \\ fs [MEM_SPLIT, list_size_APPEND, list_size_def]
 End
 
+Definition has_res_mod_name_def:
+  (* TODO: check this string code translates to something sane *)
+  has_res_mod_name mnm = (compiler_module_name ≼ mnm)
+End
+
+Definition must_adj_id_def:
+  must_adj_id (Short nm) = F ∧
+  must_adj_id (Long mnm id) = (has_res_mod_name mnm ∨ must_adj_id id)
+End
+
+Definition must_adj_pat_def:
+  (must_adj_pat (Pcon id ps) = ((case id of SOME c => must_adj_id c | _ => F) ∨
+        EXISTS must_adj_pat ps)) ∧
+  (must_adj_pat (Pref p) = must_adj_pat p) ∧
+  (must_adj_pat (Ptannot p t) = must_adj_pat p) ∧
+  (must_adj_pat p = F)
+Termination
+  WF_REL_TAC `measure pat_size`
+  \\ simp_tac bool_ss [GSYM size_abbrevs, pats_size_thm]
+  \\ rw []
+  \\ fs [MEM_SPLIT, SUM_APPEND]
+End
+
+Definition must_adj_exp_def:
+  (must_adj_exp (Var id) = must_adj_id id) ∧
+  (must_adj_exp (Raise e) = must_adj_exp e) ∧
+  (must_adj_exp (Handle e pes) = (must_adj_exp e ∨
+        (EXISTS (\(p, x). must_adj_pat p ∨ must_adj_exp x) pes))) ∧
+  (must_adj_exp (Con cn es) = ((case cn of SOME c => must_adj_id c | _ => F) ∨
+        EXISTS must_adj_exp es)) ∧
+  (must_adj_exp (Fun x e) = must_adj_exp e) ∧
+  (must_adj_exp (App op es) = (op = Eval ∨ EXISTS must_adj_exp es)) ∧
+  (must_adj_exp (Log lop e1 e2) = (must_adj_exp e1 ∨ must_adj_exp e2)) ∧
+  (must_adj_exp (If e1 e2 e3) = (must_adj_exp e1 ∨ must_adj_exp e2 ∨
+        must_adj_exp e3)) ∧
+  (must_adj_exp (Mat e pes) = (must_adj_exp e ∨
+        (EXISTS (\(p, x). must_adj_pat p ∨ must_adj_exp x) pes))) ∧
+  (must_adj_exp (Let nm e1 e2) = (must_adj_exp e1 ∨ must_adj_exp e2)) ∧
+  (must_adj_exp (Letrec funs e) = (must_adj_exp e ∨
+    (EXISTS (\(a, b, x). must_adj_exp x) funs))) ∧
+  (must_adj_exp (Tannot x t) = must_adj_exp x) ∧
+  (must_adj_exp (Lannot x locs) = must_adj_exp x)
+Termination
+  WF_REL_TAC `measure exp_size`
+  \\ rw [exp_size_def]
+  \\ fs (map (REWRITE_RULE [size_abbrevs])
+    [funs_size_thm, pes_size_thm, exps_size_thm])
+  \\ fs [MEM_MAP, EXISTS_PROD]
+  \\ fs [MEM_SPLIT, exp_size_def, SUM_APPEND]
+End
+
+Definition must_adj_type_def:
+  (must_adj_type (Atapp ts id) <=> must_adj_id id ∨ EXISTS must_adj_type ts) /\
+  (must_adj_type (Attup ts) = EXISTS must_adj_type ts) /\
+  (must_adj_type (Atfun t1 t2) <=> must_adj_type t1 ∨ must_adj_type t2) /\
+  (must_adj_type t = F)
+Termination
+  WF_REL_TAC `measure ast_t_size`
+  \\ rw [ast_t_size_def, ast_t1_size]
+  \\ fs [MEM_SPLIT, ast_t_size_def, SUM_APPEND]
+End
+
+Definition must_adj_dec_def:
+  (must_adj_dec (Dlet loc nm e) = must_adj_exp e) ∧
+  (must_adj_dec (Dletrec locs funs) =
+        EXISTS (\(a, b, x). must_adj_exp x) funs) ∧
+  (must_adj_dec (Dmod mnm ds) <=> has_res_mod_name mnm ∨
+        EXISTS must_adj_dec ds) ∧
+  (must_adj_dec (Dlocal lds ds) <=> EXISTS must_adj_dec lds ∨
+        EXISTS must_adj_dec ds) ∧
+  (must_adj_dec (Dexn locs cn ts) = EXISTS must_adj_type ts) ∧
+  (must_adj_dec (Dtabbrev locs vs nm t) = must_adj_type t) ∧
+  (must_adj_dec (Dtype locs td) = 
+        EXISTS (EXISTS (EXISTS must_adj_type o SND) o SND o SND) td) ∧
+  (must_adj_dec d = F)
+Termination
+  WF_REL_TAC `measure dec_size`
+  \\ rw [dec_size_def, dec1_size_eq]
+  \\ fs [MEM_SPLIT, list_size_APPEND, list_size_def]
+End
+
+Definition fast_compile_dec_def:
+  fast_compile_dec dec = if must_adj_dec dec then compile_dec dec else dec
+End
+
 Definition compile_def:
   compile cfg decs = if EXISTS has_Eval_dec decs
-    then compiler_module cfg :: MAP compile_dec decs
+    then compiler_module cfg :: MAP fast_compile_dec decs
     else decs
 End
 
